ok

CNF_chomsky.thy
@@ -16,9 +16,9 @@ definition Productions :: "('n, 't)RuleSet \<Rightarrow> (('n, 't)PartialEvaluat
 definition ProductionStep :: "('n, 't) PartialEvaluation \<Rightarrow> ('n, 't)RuleSet \<Rightarrow> ('n, 't)PartialEvaluation \<Rightarrow> bool"  ("_ -_\<rightarrow> _" [60, 61, 60] 61) 
   where "w -G\<rightarrow> w' \<equiv> (w, w') \<in> Productions G"
 
-fun ProducesInN :: "('n, 't) PartialEvaluation \<Rightarrow> ('n, 't) RuleSet \<Rightarrow> nat \<Rightarrow> ('n, 't) PartialEvaluation \<Rightarrow> bool" ("_ -_\<rightarrow>\<^sup>_ _" [60, 61, 61, 60] 61)
+fun ProducesInN :: "('n, 't) PartialEvaluation \<Rightarrow> ('n, 't) RuleSet \<Rightarrow> nat \<Rightarrow> ('n, 't) PartialEvaluation \<Rightarrow> bool" ("_ -_\<rightarrow>\<^sup>_ _" [60, 61, 62, 60] 61)
   where "s -G\<rightarrow>\<^sup>0 t = (s = t)" | 
-        "ProducesInN s G (Suc(n)) t = (\<exists> r. s -G\<rightarrow> r \<and> s -G\<rightarrow>\<^sup>n t)"
+        "ProducesInN s G (Suc(n)) t = (\<exists> r. s -G\<rightarrow> r \<and> r -G\<rightarrow>\<^sup>n t)"
 
 definition Produces :: "('n, 't) PartialEvaluation \<Rightarrow> ('n, 't) RuleSet \<Rightarrow> ('n, 't) PartialEvaluation \<Rightarrow> bool" ("_ -_\<rightarrow>\<^sup>* _" [60, 61, 60] 61) 
   where "w -G\<rightarrow>\<^sup>* w' \<equiv> \<exists> n. w -G\<rightarrow>\<^sup>n w'"
@@ -26,8 +26,11 @@ definition Produces :: "('n, 't) PartialEvaluation \<Rightarrow> ('n, 't) RuleSe
 definition IsTerminalWord :: "('n, 't) Elem list \<Rightarrow> bool"
   where "IsTerminalWord El \<equiv> \<not>(\<exists> a. NT(a) \<in> set El)"
 
+definition PartialEvalLanguage :: "('n, 't) Elem list \<Rightarrow> ('n, 't) RuleSet \<Rightarrow> (('n, 't) Elem list) set"
+  where "PartialEvalLanguage E R = { w | w. IsTerminalWord w \<and> E -R\<rightarrow>\<^sup>* w}"
+
 definition Language :: "'n \<Rightarrow> ('n, 't) RuleSet \<Rightarrow> (('n, 't) Elem list) set" ("\<lbrakk>_\<rbrakk>\<^sub>_" [60, 61])
-  where "\<lbrakk>S\<rbrakk>\<^sub>G = { w | w. IsTerminalWord w \<and> [NT(S)] -G\<rightarrow>\<^sup>* w}"
+  where "\<lbrakk>S\<rbrakk>\<^sub>G = PartialEvalLanguage [NT S] G"
 
 definition Lang :: "('n, 't) CFG \<Rightarrow> (('n, 't) Elem list) set" ("\<lbrakk>_\<rbrakk>")
   where "Lang G \<equiv> {w | w S R. w \<in> \<lbrakk>S\<rbrakk>\<^sub>R \<and> (S, R) = G}"
@@ -36,7 +39,7 @@ definition NTInRule :: "'n \<Rightarrow> ('n, 't) Rule \<Rightarrow> bool"
   where "NTInRule N R \<equiv> \<exists> S Rhs. (S, Rhs) = R \<and> (S = N \<or> (NT(N) \<in> set Rhs))"
 
 definition NonTerminals :: "('n, 't) CFG \<Rightarrow> ('n, 't) Elem set"
-  where "NonTerminals G = {NT(a) | S Rs a R. (S, Rs) = G \<and> R \<in> Rs \<and> NTInRule a R}"
+  where "NonTerminals G = {NT(a) | S Rs a R. (S, Rs) = G \<and> (R \<in> Rs \<and> NTInRule a R \<or> S = a)}"
 
 definition ProducingNT :: "('n, 't) Rule \<Rightarrow> 'n"
   where "ProducingNT R = fst R"
@@ -47,6 +50,429 @@ definition TInRule ::  "'t \<Rightarrow> ('n, 't) Rule \<Rightarrow> bool"
 definition Terminals :: "('n, 't) CFG \<Rightarrow> ('n, 't) Elem set"
   where "Terminals G = {T(a) | S Rs a R. (S, Rs) = G \<and> R \<in> Rs \<and> TInRule a R}"
 
+section "Basic properties"
+
+lemma productionSum:
+  assumes a: "A -R\<rightarrow>\<^sup>n B"
+  assumes b: "B -R\<rightarrow>\<^sup>m C"
+  shows      "ProducesInN A R (n+m) C"
+proof-
+  have 0: "\<And> A B C m. A -R\<rightarrow>\<^sup>n B \<and> B -R\<rightarrow>\<^sup>m C \<Longrightarrow> ProducesInN A R (n+m) C"
+    by(induction n, auto)
+  from 0 show ?thesis 
+    using a b by force
+qed
+
+lemma productionAppend1:
+  assumes a: "N -R\<rightarrow> P"
+  shows      "(l @ N @ r) -R\<rightarrow> (l @ P @ r)"
+proof-
+  from a show ?thesis
+    apply(unfold ProductionStep_def Productions_def)
+    by (smt (verit, best) Pair_inject append.assoc mem_Collect_eq)
+qed
+
+lemma productionAppend2:
+  assumes a: "N -R\<rightarrow>\<^sup>n P"
+  shows      "(l @ N @ r) -R\<rightarrow>\<^sup>n (l @ P @ r)"
+proof-
+  from productionAppend1 have 0: "\<And> N R P l r. ((N -R\<rightarrow>\<^sup>n P) \<Longrightarrow> (l @ N @ r) -R\<rightarrow>\<^sup>n (l @ P @ r))"
+    by(induction n, auto, blast)
+  from 0 show ?thesis
+    using assms by blast
+qed
+
+lemma productionAppend3:
+  assumes a: "N -R\<rightarrow>\<^sup>* P"
+  shows      "(l @ N @ r) -R\<rightarrow>\<^sup>* (l @ P @ r)"
+proof-
+  from a have 0: "\<exists> n. N -R\<rightarrow>\<^sup>n P" (is "\<exists> n. ?P n")
+    by (simp add: Produces_def)
+  then obtain n where 1: "?P n" by blast
+  from 1 and productionAppend2 show ?thesis
+    apply(unfold Produces_def)
+    by blast
+qed
+
+lemma transitiveProductions:
+  assumes a: "a -R\<rightarrow>\<^sup>* b"
+  assumes b: "b -R\<rightarrow>\<^sup>* c"
+  shows      "a -R\<rightarrow>\<^sup>* c"
+proof-  
+  from a have 0: "\<exists> n. a -R\<rightarrow>\<^sup>n b" (is "\<exists> n. ?P n")
+    by (simp add: Produces_def)
+  then obtain n where 1: "?P n" by blast
+  from b have 2: "\<exists> m. b -R\<rightarrow>\<^sup>m c" (is "\<exists> m. ?P m")
+    by (simp add: Produces_def)
+  then obtain m where 3: "?P m" by blast
+  have 4: "\<And> a b. a -R\<rightarrow>\<^sup>n b \<and> b -R\<rightarrow>\<^sup>m c \<Longrightarrow> ProducesInN a R (n+m) c"
+    by(induction n, auto)
+  from 4 and 1 and 3 show ?thesis apply(unfold Produces_def) 
+    by blast
+qed
+
+lemma listPrefixSize:
+  assumes a: "l @ r = a @ b"
+  assumes b: "size l \<ge> size a"
+  shows      "\<exists> c. l = a @ c"
+proof-
+  from a and b show ?thesis
+    by (metis append_eq_append_conv_if append_eq_conv_conj)
+qed
+
+lemma listSuffixSize:
+  assumes a: "l @ r = a @ b"
+  assumes b: "size r \<ge> size b"
+  shows      "\<exists> c. r = c @ b"
+proof-
+  from a and b show ?thesis
+    by (smt (verit, ccfv_SIG) add_mono_thms_linordered_semiring(3) append_eq_append_conv append_eq_append_conv_if length_append verit_la_disequality)
+qed
+
+lemma productionParts1:
+  assumes a: "l @ r -R\<rightarrow> X"
+  shows      "(\<exists> l'. l -R\<rightarrow> l' \<and> l' @ r = X) \<or> (\<exists> r'. r -R\<rightarrow> r' \<and> l @ r' = X)"   
+proof-
+  from a have 0: "\<exists> N rhs a b. l @ r = (a @ [NT N] @ b) \<and> X = (a @ rhs @ b) \<and> (N, rhs) \<in> R" (is "\<exists> N rhs a b. ?P N rhs a b")
+    by (smt (verit) Pair_inject ProductionStep_def Productions_def mem_Collect_eq)
+  then obtain N rhs a b where 1: "?P N rhs a b" by blast
+  from 1 have 3: "(size l \<ge> size (a @ [NT N])) \<Longrightarrow> \<exists> c. l = (a @ [NT N]) @ c"
+    by (metis append.assoc listPrefixSize)
+  have 4: "size l > size a \<Longrightarrow> size l \<ge> size (a @ [NT N])"
+    by simp
+  from 1 have 5: "size l + size r = size a + size ([NT N] @ b)"
+    by (metis length_append)
+  from 5 have 6: "size l \<le> size a \<Longrightarrow> size r \<ge> size ([NT N] @ b)"
+    by linarith
+  from 1 have 7: "size r \<ge> size ([NT N] @ b) \<Longrightarrow> \<exists> c. r = c @ ([NT N] @ b)"
+    by (metis listSuffixSize)
+  have 2: "((size l) > (size a)) \<or> ((size l) \<le> size a)"
+    using linorder_not_less by blast
+  then show ?thesis
+  proof
+    assume x: "(size l) > (size a)"
+    from x and 4 have 8: "size l \<ge> size (a @ [NT N])"
+      by auto
+    from 8 and 3 have 9:"\<exists> c. l = (a @ [NT N]) @ c" (is "\<exists> c. ?P c")
+      by auto
+    then obtain c where 10: "?P c" by blast
+    from 10 and 1 have 11: "l -R\<rightarrow> (a @ rhs @ c)"
+      apply(unfold ProductionStep_def, auto) 
+      using Productions_def by fastforce
+    from 10 and 1 have 12: "c @ r = b" by simp
+    from 1 and 12 and 11 have 13: "\<exists> l'. l -R\<rightarrow> l' \<and> l' @ r = X"
+      by force
+    show ?thesis
+      by (simp add: "13")
+  next
+    assume y: "((size l) \<le> size a)"
+    from y and 6 have 8: "size r \<ge> size ([NT N] @ b)"
+      by auto
+    from 8 and 7 have 9: "\<exists> c. r = c @ ([NT N] @ b)" (is "\<exists> c. ?P c")
+      by auto
+    then obtain c where 10: "?P c" by blast
+    from 10 and 1 have 11: "r -R\<rightarrow> (c @ rhs @ b)"
+      apply(unfold ProductionStep_def, auto) 
+      using Productions_def by fastforce
+    from 10 and 1 have 12: "l @ c = a" by simp
+    from 1 and 12 and 11 have 13: "(\<exists> r'. r -R\<rightarrow> r' \<and> l @ r' = X)"
+      by force
+    show ?thesis
+      by (simp add: "13")
+  qed
+qed  
+
+lemma ProductionParts2:
+  assumes a: "(\<And>X l r. l @ r -R\<rightarrow>\<^sup>n X \<Longrightarrow> \<exists>l' r'. l -R\<rightarrow>\<^sup>* l' \<and> r -R\<rightarrow>\<^sup>* r' \<and> l' @ r' = X)"
+  assumes b: "ProducesInN (l@r) R (Suc(n)) X"
+  shows      "\<exists>l' r'. l -R\<rightarrow>\<^sup>* l' \<and> r -R\<rightarrow>\<^sup>* r' \<and> l' @ r' = X"
+proof-
+  from b have 0: "\<exists> q. l@r -R\<rightarrow> q \<and> q -R\<rightarrow>\<^sup>n X" (is "\<exists> q. ?P q")
+    by auto  
+  then obtain q where 1 : "?P q" by blast
+  from 1 and productionParts1 have 2:"(\<exists> l'. l -R\<rightarrow> l' \<and> l' @ r = q) \<or> (\<exists> r'. r -R\<rightarrow> r' \<and> l @ r' = q)"
+    by metis
+  have 3: "\<And> x. x -R\<rightarrow>\<^sup>0 x" 
+    by simp
+  from 3 have 4: "\<And> x. x -R\<rightarrow>\<^sup>* x" 
+    using Produces_def by blast
+  from 2 and 4 have 5: "\<exists> l' r'. q = l' @ r' \<and> l -R\<rightarrow>\<^sup>* l' \<and>  r -R\<rightarrow>\<^sup>* r'"
+    by (meson ProducesInN.simps(1) ProducesInN.simps(2) Produces_def)
+  from 5 and 1 show ?thesis
+    by (smt (z3) "2" ProducesInN.simps(2) Produces_def a)
+qed
+
+lemma productionParts3:
+  assumes a: "l @ r -R\<rightarrow>\<^sup>* X"
+  shows      "\<exists> l' r'. l -R\<rightarrow>\<^sup>* l' \<and> r -R\<rightarrow>\<^sup>* r' \<and> l' @ r' = X"
+proof-
+  from a have 0: "\<exists> n. l @ r -R\<rightarrow>\<^sup>n X" (is "\<exists> n. ?P n")
+    by (simp add: Produces_def)
+  then obtain n where 1: "?P n" by blast
+  have 2: "\<And> X l r. l @ r -R\<rightarrow>\<^sup>n X \<Longrightarrow> \<exists> l' r'. l -R\<rightarrow>\<^sup>* l' \<and> r -R\<rightarrow>\<^sup>* r' \<and> l' @ r' = X"
+    apply(induction n)
+    apply (meson ProducesInN.simps(1) Produces_def)
+    using ProductionParts2 by blast
+  from 2 and 1 show ?thesis
+    by force
+qed
+
+lemma productionParts4:
+  assumes a: "l -R\<rightarrow>\<^sup>* l'"
+  assumes b: "r -R\<rightarrow>\<^sup>* r'"
+  shows      "l @ r -R\<rightarrow>\<^sup>* l' @ r'"
+proof-
+  from a and productionAppend3 have 0: "l @ r -R\<rightarrow>\<^sup>* l' @ r"
+    by (metis append_Nil)
+  from b and productionAppend3 have 1: "l' @ r -R\<rightarrow>\<^sup>* l' @ r'"
+    by (metis append.right_neutral)
+  from 0 and 1 show ?thesis 
+    using transitiveProductions by blast
+qed
+
+lemma productionParts5:
+  assumes a: "\<And> l r X. l @ r -R\<rightarrow>\<^sup>n X \<Longrightarrow> \<exists>l' r' m. n \<ge> m \<and> l -R\<rightarrow>\<^sup>m l' \<and> ProducesInN r R (n-m) r' \<and> l' @ r' = X"
+  assumes b: "ProducesInN (l @ r) R (n+1) X"
+  shows      "\<exists>l' r' m. (n+1) \<ge> m \<and> l -R\<rightarrow>\<^sup>m l' \<and> ProducesInN r R ((n+1)-m) r' \<and> l' @ r' = X"
+proof-
+  from b have 0: "\<exists> t. (l @ r) -R\<rightarrow> t \<and> t -R\<rightarrow>\<^sup>n X" (is "\<exists> t. ?P t")
+    by auto
+  then obtain t where 1: "?P t" by blast
+  from 1 and productionParts1 have 2: "(\<exists> l'. l -R\<rightarrow> l' \<and> l' @ r = t) \<or> (\<exists> r'. r -R\<rightarrow> r' \<and> l @ r' = t)"
+    by blast
+  then show ?thesis
+  proof 
+    assume "(\<exists> l1. l -R\<rightarrow> l1 \<and> l1 @ r = t)" (is "\<exists> l1. ?P l1")
+    then obtain l1 where 3: "?P l1" by blast
+    from 0 and 1 and a and 3 have 4: "\<exists>l' r' m. n \<ge> m \<and> l1 -R\<rightarrow>\<^sup>m l' \<and> ProducesInN r R (n-m) r' \<and> l' @ r' = X" (is "\<exists> l' r' m. ?P l' r' m")
+      by simp
+    then obtain l' r' m where 5: "?P l' r' m" by blast
+    from 5 and 3 have 6: "ProducesInN l R (m+1) l'"
+      by (metis ProducesInN.simps(2) Suc_eq_plus1)
+    from 5 and 6 show ?thesis
+      by(rule_tac x="l'" in exI, rule_tac x="r'" in exI, rule_tac x="m+1" in exI, auto)
+  next
+    assume "(\<exists> r1. r -R\<rightarrow> r1 \<and> l @ r1 = t)" (is "\<exists> r1. ?P r1")
+    then obtain r1 where 3: "?P r1" by blast
+    from 0 and 1 and a and 3 have 4: "\<exists>l' r' m. n \<ge> m \<and> l -R\<rightarrow>\<^sup>m l' \<and> ProducesInN r1 R (n-m) r' \<and> l' @ r' = X" (is "\<exists> l' r' m. ?P l' r' m")
+      by simp
+    then obtain l' r' m where 5: "?P l' r' m" by blast
+    from 5 and 3 have 6: "ProducesInN r R (n-m+1) r'"
+      by (metis ProducesInN.simps(2) Suc_eq_plus1)
+    from 6 have 7:  "ProducesInN r R (n+1-m) r'"
+      by (metis "5" Nat.add_diff_assoc2)
+    from 5 and 7 show ?thesis
+      by(rule_tac x="l'" in exI, rule_tac x="r'" in exI, rule_tac x="m" in exI, auto)
+  qed
+qed
+
+lemma productionParts6:
+  assumes a: "l @ r -R\<rightarrow>\<^sup>n X"
+  shows      "\<exists> l' r' m. n \<ge> m \<and> l -R\<rightarrow>\<^sup>m l' \<and> ProducesInN r R (n-m) r' \<and> l' @ r' = X"
+proof- 
+  from productionParts5 have 0: "\<And>l r X n. ((\<And>l r X. l @ r -R\<rightarrow>\<^sup>n X \<Longrightarrow> 
+           \<exists>l' r' m. m \<le> n \<and> l -R\<rightarrow>\<^sup>m l' \<and> ProducesInN r R (n-m) r' \<and> l' @ r' = X) \<Longrightarrow>
+           (ProducesInN (l@r) R (n+1) X) \<Longrightarrow> 
+            \<exists>l' r' m. m \<le> n + 1 \<and> l -R\<rightarrow>\<^sup>m l' \<and> (ProducesInN r R ((n+1)-m) r') \<and> l' @ r' = X)"
+       by blast
+  have 1: "\<And> l r X. l @ r -R\<rightarrow>\<^sup>n X \<Longrightarrow> \<exists> l' r' m. n \<ge> m \<and> l -R\<rightarrow>\<^sup>m l' \<and> ProducesInN r R (n-m) r' \<and> l' @ r' = X"
+    apply(induction n) apply simp 
+    using "0" by auto
+  from 1 show ?thesis
+    using assms by blast
+qed
+
+lemma productionParts7:
+  assumes a: "l -R\<rightarrow>\<^sup>n l'"
+  assumes b: "r -R\<rightarrow>\<^sup>m r'"
+  shows      "ProducesInN (l @ r) R (n+m) (l' @ r')"
+proof- 
+  from a and productionAppend2 have 0: "ProducesInN (l @ r) R (n) (l' @ r)"
+    by (metis append_Nil)
+  from b have 1: "ProducesInN (l' @ r) R m (l' @ r')"
+    by (metis append.right_neutral productionAppend2)
+  from 0 and 1 and productionSum show ?thesis
+    by blast
+qed
+
+lemma RuleSubset1:
+  fixes      Rs1 :: "('n, 't) RuleSet"
+  fixes      Rs2 :: "('n, 't) RuleSet"
+  assumes a: "Rs1 \<subseteq> Rs2"
+  assumes b: "S -Rs1\<rightarrow> X"
+  shows      "S -Rs2\<rightarrow> X"
+proof-
+  from a and b show ?thesis
+    by(unfold ProductionStep_def Productions_def, blast)
+qed
+
+lemma RuleSubset:
+  fixes      Rs1 :: "('n, 't) RuleSet"
+  fixes      Rs2 :: "('n, 't) RuleSet"  
+  fixes      S :: "'n"
+  assumes a: "Rs1 \<subseteq> Rs2"
+  assumes b: "x \<in> Language S Rs1"
+  shows      "x \<in> Language S Rs2"
+proof-
+  from b have 0: "\<exists>n. ([NT S]) -Rs1\<rightarrow>\<^sup>n x" (is "\<exists>n. ?P n")
+    by(unfold Language_def PartialEvalLanguage_def Produces_def, auto)
+  then obtain n where 1: "?P n" by blast
+  from b have 2: "IsTerminalWord x"
+    by (unfold Language_def PartialEvalLanguage_def Produces_def, auto)
+  from a and RuleSubset1 have 3: "\<And> S x. S -Rs1\<rightarrow>\<^sup>n x \<Longrightarrow> S -Rs2\<rightarrow>\<^sup>n x"
+    apply(induction n, auto, simp)
+    by blast
+  from 3 and 1 and 2 show ?thesis
+    apply(unfold Language_def PartialEvalLanguage_def Produces_def, auto)
+    done
+qed
+
+lemma OrderInvariant_Part1:
+  fixes      Rs :: "('n, 't) RuleSet"
+  fixes      P :: "('n, 't) Elem list"
+  assumes a: "L = PartialEvalLanguage P Rs"
+  assumes b: "P = l @ [NT N] @ r"
+  assumes c: "Ls = {PartialEvalLanguage (l @ rhs @ r) Rs | rhs. (N, rhs) \<in> Rs}"
+  assumes d: "x \<in> (\<Union> Ls)"
+  shows      "x \<in> L"
+proof-
+  from c and d have 0: "\<exists> Rhs. (N, Rhs) \<in> Rs \<and> x \<in> PartialEvalLanguage (l @ Rhs @ r) Rs" (is "\<exists> Rhs. ?P Rhs")
+    by blast
+  then obtain Rhs where 1: "?P Rhs" by blast
+  from 1 have 2: "(N, Rhs) \<in> Rs" by auto
+  from 2 have 3: "[NT N] -Rs\<rightarrow> Rhs" 
+    apply (simp add: ProductionStep_def Productions_def) 
+    by fastforce
+  from b and 3 and productionAppend1 have 4: "P -Rs\<rightarrow> (l @ Rhs @ r)" 
+    by blast
+  from 4 have 5: "PartialEvalLanguage (l @ Rhs @ r) Rs \<subseteq> PartialEvalLanguage P Rs"
+    apply(unfold PartialEvalLanguage_def Produces_def)
+    by (smt (verit) Collect_mono ProducesInN.simps(2))
+  from a and b and c and d and 5 and 1 show ?thesis
+    by blast
+qed
+
+lemma OrderInvariant_Part2:
+  fixes      Rs :: "('n, 't) RuleSet"
+  fixes      P :: "('n, 't) Elem list"
+  assumes a: "L = PartialEvalLanguage P Rs"
+  assumes b: "P = l @ [NT N] @ r"
+  assumes c: "Ls = {PartialEvalLanguage (l @ rhs @ r) Rs | rhs. (N, rhs) \<in> Rs}"
+  assumes d: "x \<in> L"
+  shows      "x \<in> \<Union> Ls"
+proof-
+  from d and a have 0: "\<exists> n. P -Rs\<rightarrow>\<^sup>n x" (is "\<exists>n. ?P n")
+    by(unfold PartialEvalLanguage_def Produces_def, auto)
+  then obtain n where 1: "?P n" by blast
+  from d and a have 2: "IsTerminalWord x"
+    by(unfold PartialEvalLanguage_def Produces_def, auto)
+  from b and a and d and productionParts3 have 3: "\<exists> ln r'. l @ [NT N] -Rs\<rightarrow>\<^sup>* ln \<and> r -Rs\<rightarrow>\<^sup>* r' \<and> x = ln@r'" (is "\<exists> ln r'. ?P ln r'")
+    by (metis "0" Produces_def append_assoc)
+  then obtain ln r' where 4: "?P ln r'" by blast
+  from 4 have 5: "\<exists> l' rhs. l -Rs\<rightarrow>\<^sup>* l' \<and> [NT N]-Rs\<rightarrow>\<^sup>* rhs \<and> ln = l' @ rhs" (is "\<exists> l' rhs. ?P l' rhs")
+    using productionParts3 by blast
+  then obtain l' rhs where 6: "?P l' rhs" by blast
+  from 4 and 6 have 7: "x = l' @ rhs @ r'" by auto
+  from 6 have 8: "\<exists> k. [NT N] -Rs\<rightarrow>\<^sup>k rhs" (is "\<exists>k. ?P k") 
+    by (unfold Produces_def, auto) 
+  then obtain k where 9: "?P k" by blast
+  from 9 and 2 have 10: "k \<ge> 1"
+    using "7" IsTerminalWord_def in_set_conv_decomp not_less_eq_eq by fastforce
+  from 10 and 8 have 11: "\<exists> rht. [NT N] -Rs\<rightarrow> rht \<and> ProducesInN rht Rs (k-1) rhs" (is "\<exists> rht. ?P rht")
+    using "9" ProducesInN.elims(2) by fastforce
+  then obtain rht where 12: "?P rht" by blast
+  from 12 and 10 have 13: "rht -Rs\<rightarrow>\<^sup>* rhs"
+    using Produces_def by blast 
+  from 12 have 14: "l @ [NT N] @ r -Rs\<rightarrow> l @ rht @ r" 
+    using productionAppend1 by blast
+  from 13 have 15: "l @ rht @ r -Rs\<rightarrow>\<^sup>* l @ rhs @ r" 
+    using productionAppend3 by blast
+  from 15 and 13 and 4 and 6 have 16: "l @ rht @ r -Rs\<rightarrow>\<^sup>* l' @ rhs @ r'"
+    by (simp add: productionParts4)
+  from 16 and 7 have 17: "l @ rht @ r -Rs\<rightarrow>\<^sup>* x" by auto
+  from 17 and 2 have 18: "x \<in> PartialEvalLanguage (l @ rht @ r) Rs" 
+    using PartialEvalLanguage_def by blast
+  from 12 have 19: "[NT N] -Rs\<rightarrow> rht" by auto
+  from 19 have 20: "\<exists> lt rt rhst Nt. (lt @ [NT Nt] @ rt, lt @ rhst @ rt) = ([NT N], rht) \<and> (Nt, rhst) \<in> Rs" (is "\<exists> lt rt rhst Nt. ?P lt rt rhst Nt")
+    apply(unfold ProductionStep_def Productions_def) 
+    by fastforce
+  then obtain lt rt rhst Nt where 21: "?P lt rt rhst Nt" by blast
+  from 21 have 22: "lt = [] \<and> rt = [] \<and> N = Nt" 
+    by (simp add: append_eq_Cons_conv)
+  from 21 and 22 have 23: "rhst = rht" by auto
+  from 21 and 22 and 23 have 24: "(N, rht) \<in> Rs" by auto
+  from 12 and 24 have 25: "PartialEvalLanguage (l @ rht @ r) Rs \<in> Ls"
+    using c by blast
+  from 18 and 25 show ?thesis
+    by blast
+qed
+  
+lemma OrderInvariant:
+  fixes      Rs :: "('n, 't) RuleSet"
+  fixes      P :: "('n, 't) Elem list"
+  fixes      l :: "('n, 't) Elem list"
+  fixes      r :: "('n, 't) Elem list"
+  fixes      L :: "('n, 't) Elem list set"
+  fixes      Ls :: "('n, 't) Elem list set set"
+  fixes      N :: "'n"
+  assumes a: "L = PartialEvalLanguage P Rs"
+  assumes b: "P = l @ [NT N] @ r"
+  assumes c: "Ls = {PartialEvalLanguage (l @ rhs @ r) Rs | rhs. (N, rhs) \<in> Rs}"
+  shows      "\<Union> Ls = L"
+proof-
+  from a and b and c and OrderInvariant_Part1 have 0: "\<And> x. (x \<in> \<Union> Ls \<Longrightarrow> x \<in> L)"
+    by fastforce
+  from a and b and c and OrderInvariant_Part2 have 1: "\<And> x. (x \<in> L \<Longrightarrow> x \<in> \<Union> Ls)"
+    by fastforce
+  from 0 and 1 show ?thesis by blast
+qed  
+
+lemma OrderInvStep: 
+  fixes      Rs :: "('n, 't) RuleSet"
+  fixes      P :: "('n, 't) Elem list"
+  fixes      l :: "('n, 't) Elem list"
+  fixes      r :: "('n, 't) Elem list"
+  fixes      N :: "'n"
+  fixes      n :: "nat"
+  assumes a: "P = l @ [NT N] @ r"
+  assumes b: "P -Rs\<rightarrow>\<^sup>n x"
+  assumes c: "IsTerminalWord x"
+  shows      "\<exists> rhs. (N, rhs) \<in> Rs \<and> ProducesInN (l @ rhs @ r) Rs (n-1) x" 
+proof-
+  from b and productionParts6 have 0: "\<exists> l' nr a. n \<ge> a \<and> l -Rs\<rightarrow>\<^sup>a l' \<and> ProducesInN ([NT N] @ r) Rs (n-a) nr \<and> l' @ nr = x"
+    (is "\<exists> l' nr a. ?P l' nr a")
+    using a by blast
+  then obtain l' nr a where 1: "?P l' nr a" by blast
+  from 1 have 2: "\<exists> N' r' b. n-a \<ge> b \<and> [NT N] -Rs\<rightarrow>\<^sup>b N' \<and> ProducesInN (r) Rs (n-a-b) r' \<and>  N' @ r' = nr"
+    (is "\<exists> N' r' b. ?P N' r' b")
+    by (meson diff_le_self le_trans productionParts6)
+  then obtain N' r' b where 3: "?P N' r' b" by blast
+  from c and 3 have 4: "N' \<noteq> [NT N]" 
+    by (metis "1" IsTerminalWord_def append_Cons in_set_conv_decomp)
+  from 4 and 3 and c have 5: "b \<ge> 1"
+    by (metis One_nat_def ProducesInN.simps(1) Suc_leI bot_nat_0.not_eq_extremum)
+  from 3 and 5 have 6: "\<exists> t. [NT N] -Rs\<rightarrow> t \<and> ProducesInN t Rs (b-1) N'" 
+    (is "\<exists> t. ?P t")
+    by (metis "4" ProducesInN.elims(2) diff_Suc_1)
+  then obtain t where 7: "?P t" by blast
+  from 7 and 3 and productionParts7 have 8: "ProducesInN (t @ r) Rs ((n-a-b)+(b-1)) nr"
+    by (metis add.commute)
+  from 8 and 1 and productionParts7 have 9: "ProducesInN (l @ t @ r) Rs ((n-a-b)+(b-1)+a) x"
+    by (metis add.commute)
+  from 1 and 3 have 10: "(n-a-b)+(b-1)+a = n-1"
+    using "5" by force
+  from 10 and 9 have 11: "ProducesInN (l @ t @ r) Rs (n-1) x" by auto
+  from 7 have 12: "\<exists> ln rn Nn rhs. [NT N] = ln @ [NT Nn] @ rn \<and> t = ln @ rhs @ rn \<and> (Nn, rhs) \<in> Rs" (is "\<exists> ln rn Nn rhs. ?P  ln rn Nn rhs")
+    apply(unfold ProductionStep_def Productions_def) 
+    by blast
+  then obtain ln rn Nn rhs where 13: "?P ln rn Nn rhs" by blast
+  from 13 have 14: "ln = [] \<and> rn = [] \<and> Nn = N \<and> rhs = t"
+    by (simp add: Cons_eq_append_conv)
+  from 14 13 have 15: "(N, t) \<in> Rs" by auto
+  from 11 and 15 show ?thesis by auto
+qed
+
+
 definition transformStart :: "('n, 't) CFG \<Rightarrow> 'n \<Rightarrow> ('n, 't) CFG \<Rightarrow> bool" 
   where "transformStart G1 S0 G2 \<equiv> \<exists> S1 R1 R2. (S1, R1) = G1 
                                    \<and> (S0, R2) = G2 
@@ -54,37 +480,131 @@ definition transformStart :: "('n, 't) CFG \<Rightarrow> 'n \<Rightarrow> ('n, '
                                    \<and> R2 = insert (S0, [NT(S1)]) R1"
 
 lemma Start_Part1:
-    assumes a: "transformStart (S1, R1) S0 (S0, insert (S0, [NT S1]) R1)"
-    assumes b: "\<forall>a. NT a \<notin> set x"
-    assumes c: "G1 = (S1, R1)"
-    assumes d: "[NT S1] -R1\<rightarrow>\<^sup>n x"
-    assumes e: "\<forall>a b. (a, b) \<in> R1 \<longrightarrow> a \<noteq> S0 \<and> NT S0 \<notin> set b" 
-    assumes f: "G2 = (S0, insert (S0, [NT S1]) R1)"
-    shows      "\<exists>n. [NT S0] -insert (S0, [NT S1]) R1\<rightarrow>\<^sup>n x"
-  using a and b and c and d and f apply-
-  apply(induction n, auto)
-  done
+  assumes a: "G1 = (S1, R1)"
+  assumes b: "G2 = (S0, R2)"
+  assumes c: "NT(S0) \<notin> NonTerminals(G1)" 
+  assumes d: "R2 = insert (S0, [NT S1]) R1"
+  assumes e: "x \<in> \<lbrakk>G1\<rbrakk>"
+  shows      "x \<in> \<lbrakk>G2\<rbrakk>"
+proof-
+  from e and a have 0: "IsTerminalWord x \<and> x \<in> Language S1 R1"
+    apply(unfold Lang_def)
+    by (simp add: Language_def PartialEvalLanguage_def)
+  from 0 and a and c and b and d and RuleSubset have 1: "[NT S1] -R2\<rightarrow>\<^sup>* x" 
+    by (metis (no_types, lifting) Language_def PartialEvalLanguage_def insertCI mem_Collect_eq subset_iff)
+  from d have 2: "[NT S0] -R2\<rightarrow> [NT S1]"
+    apply(unfold ProductionStep_def Productions_def)
+    by fastforce
+  from 2 and 1 show ?thesis 
+    apply (simp add: Lang_def Language_def PartialEvalLanguage_def Produces_def)
+    using "0" ProducesInN.simps(2) b by blast
+qed 
+
+lemma Start_Part2_induct1:
+  assumes a: "G1 = (S1, R1)"
+  assumes b: "G2 = (S0, R2)"
+  assumes c: "NT(S0) \<notin> NonTerminals(G1)" 
+  assumes d: "R2 = insert (S0, [NT S1]) R1"
+  assumes e: "(\<And>A a. (NT S0 \<notin> set A) \<and> A -R2\<rightarrow>\<^sup>n a \<Longrightarrow> A -R1\<rightarrow>\<^sup>* a)"
+  assumes f: "NT S0 \<notin> set A"
+  assumes g: "ProducesInN A R2 (Suc n) a"
+  shows      "A -R1\<rightarrow>\<^sup>* a"
+proof-
+  from a and c and b and d have 0: "\<And> R. R \<in> R2 \<Longrightarrow> R \<in> R1 \<or> R = (S0, [NT S1])"
+    by blast
+  from c have 1: "\<And> S1 Rhs1. (S1, Rhs1) \<in> R1 \<Longrightarrow> S0 \<noteq> S1 \<and> (NT S0) \<notin> set Rhs1"
+    by (smt (verit, ccfv_threshold) CollectI NTInRule_def NonTerminals_def a)
+  from 0 and 1 have 2: "\<And> Rhs. (S0, Rhs) \<in> R2 \<Longrightarrow> Rhs = [NT S1]"
+    by blast
+  from a and c and b and d and 2 have 3: "\<And> X. [NT S0] -R2\<rightarrow> X \<Longrightarrow> X = [NT S1]"
+    apply(unfold ProductionStep_def Productions_def)
+    by (smt (verit, best) Elem.inject(1) Pair_inject append_eq_Cons_conv append_is_Nil_conv list.discI list.inject mem_Collect_eq)
+  from d and 2 have 4: "\<And> A B. A \<noteq> S0 \<and> (A, B) \<in> R2 \<Longrightarrow> (A, B) \<in> R1"
+    by force
+  from 4 have 5: "\<And> A B. A -R2\<rightarrow> B \<Longrightarrow> \<exists>l r N rhs. (l @ [NT N] @ r, l @ rhs @ r) = (A, B) \<and> (N, rhs) \<in> R2"
+    by(unfold ProductionStep_def Productions_def, auto)
+  from g have 6: "\<exists> t. A -R2\<rightarrow> t \<and> t -R2\<rightarrow>\<^sup>n a" (is "\<exists> t. ?P t")
+    by simp
+  then obtain t where 7: "?P t" by blast
+  from 7 and 5 have 8: "\<exists>l r N rhs. (l @ [NT N] @ r, l @ rhs @ r) = (A, t) \<and> (N, rhs) \<in> R2" (is "\<exists> l r N rhs. ?P l r N rhs")
+    by blast
+  then obtain l r N rhs where 9: "?P l r N rhs" by blast
+  from 9 and f have 10: "N \<noteq> S0" 
+    by force
+  from 10 and 4 have 11: "(N, rhs) \<in> R1" 
+    using "9" by presburger
+  from 11 and 9 have 12: "A -R1\<rightarrow> t" 
+    using CollectI ProductionStep_def Productions_def by fastforce 
+  from 12 and 7 and e and f have 13: "t -R1\<rightarrow>\<^sup>* a"
+    by (smt (verit, ccfv_threshold) "11" "9" CollectI NTInRule_def NonTerminals_def Pair_inject Un_iff a c set_append)
+  from 12 and 13 show ?thesis 
+    by (meson ProducesInN.simps(2) Produces_def)
+qed
+
+lemma Start_Part2_induct2:
+  assumes a: "G1 = (S1, R1)"
+  assumes b: "G2 = (S0, R2)"
+  assumes c: "NT(S0) \<notin> NonTerminals(G1)" 
+  assumes d: "R2 = insert (S0, [NT S1]) R1"
+  assumes f: "NT S0 \<notin> set A"
+  assumes g: "(NT S0 \<notin> set A) \<and> A -R2\<rightarrow>\<^sup>n a"
+  shows      "A -R1\<rightarrow>\<^sup>* a"
+proof-
+  from a and b and c and d have 0: "\<And> A a. (NT S0 \<notin> set A) \<and> A -R2\<rightarrow>\<^sup>n a \<Longrightarrow>  A -R1\<rightarrow>\<^sup>* a"
+    apply(induction n)
+    apply (metis ProducesInN.simps(1) Produces_def)
+    by (metis Start_Part2_induct1 a c d)
+  from 0 and g show ?thesis
+    by blast
+qed
 
 lemma Start_Part2:
-  assumes a: "transformStart (S1, R1) S0 (S0, insert (S0, [NT S1]) R1)"
-  assumes b: "\<forall>a. NT a \<notin> set x"
-  assumes c: "G1 = (S1, R1)"
-  assumes d: "[NT S0] -insert (S0, [NT S1]) R1\<rightarrow>\<^sup>n x"
-  assumes e: "\<forall>a b. (a, b) \<in> R1 \<longrightarrow> a \<noteq> S0 \<and> NT S0 \<notin> set b" 
-  assumes f: "G2 = (S0, insert (S0, [NT S1]) R1)"
-  shows      "\<exists>n. [NT S1] -R1\<rightarrow>\<^sup>n x"
-  using a and b and c and d and f apply-
-  apply(induction n, auto)
-  done
+  assumes a: "G1 = (S1, R1)"
+  assumes b: "G2 = (S0, R2)"
+  assumes c: "NT(S0) \<notin> NonTerminals(G1)" 
+  assumes d: "R2 = insert (S0, [NT S1]) R1"
+  assumes e: "x \<in> \<lbrakk>G2\<rbrakk>"
+  shows      "x \<in> \<lbrakk>G1\<rbrakk>"
+proof-
+  from e and b have 0: "IsTerminalWord x \<and> x \<in> Language S0 R2"
+    apply(unfold Lang_def)
+    by (simp add: Language_def PartialEvalLanguage_def)
+  from 0 and b have 1: "\<exists> n. [NT S0] -R2\<rightarrow>\<^sup>n x" (is "\<exists>n. ?P n")
+    by(unfold Lang_def Language_def PartialEvalLanguage_def Produces_def, auto)
+  then obtain n where 2: "?P n" by blast
+  from a and c and b and d have 3: "\<And> R. R \<in> R2 \<Longrightarrow> R \<in> R1 \<or> R = (S0, [NT S1])"
+    by blast
+  from c have 4: "\<And> S1 Rhs1. (S1, Rhs1) \<in> R1 \<Longrightarrow> S0 \<noteq> S1 \<and> (NT S0) \<notin> set Rhs1"
+    by (smt (verit, ccfv_threshold) CollectI NTInRule_def NonTerminals_def a)
+  from 3 and 4 have 5: "\<And> Rhs. (S0, Rhs) \<in> R2 \<Longrightarrow> Rhs = [NT S1]"
+    by blast
+  from a and c and b and d and 5 have 6: "\<And> X. [NT S0] -R2\<rightarrow> X \<Longrightarrow> X = [NT S1]"
+    apply(unfold ProductionStep_def Productions_def)
+    by (smt (verit, best) Elem.inject(1) Pair_inject append_eq_Cons_conv append_is_Nil_conv list.discI list.inject mem_Collect_eq) 
+  have 7: "\<And> A a m. (NT S0 \<notin> set A) \<and> A -R2\<rightarrow>\<^sup>m a \<Longrightarrow>  A -R1\<rightarrow>\<^sup>* a"
+    by (metis Start_Part2_induct2 a c d)
+  from 6 and 0 and 1 have 8: "\<exists> r. [NT S0] -R2\<rightarrow> r \<and> ProducesInN r R2 (n-1) x"
+    by (metis "2" IsTerminalWord_def ProducesInN.elims(2) diff_Suc_1 list.set_intros(1))
+  from 8 and 6 and 7 have 9: "[NT S0] -R2\<rightarrow> [NT S1] \<and> ProducesInN [NT S1] R2 (n-1) x"
+    by force
+  from c have 10: "S1 \<noteq> S0"
+    by (simp add: NonTerminals_def a)
+  from 10 have 11: "(NT S0) \<notin> set [NT S1]"
+    by auto
+  from 9 and 7 and 11 have 12: "[NT S1] -R2\<rightarrow>\<^sup>* x"
+    using Produces_def by blast
+  from 12 show ?thesis 
+    by (metis (mono_tags, lifting) "0" "11" "7" "9" CollectI Lang_def Language_def PartialEvalLanguage_def a)
+qed
 
 theorem verifyTransformStart:
   assumes a: "transformStart G1 S0 G2"
   shows      "\<lbrakk>G1\<rbrakk> = \<lbrakk>G2\<rbrakk>"
 proof-
   from a have 1: "\<And>x. x \<in> \<lbrakk>G1\<rbrakk> \<Longrightarrow> x \<in> \<lbrakk>G2\<rbrakk>"
-    by (unfold transformStart_def NonTerminals_def NTInRule_def Lang_def Language_def Produces_def IsTerminalWord_def, auto, simp add: Start_Part1)
+    by (metis Start_Part1 transformStart_def)  
   from a have 2: "\<And>x. x \<in> \<lbrakk>G2\<rbrakk> \<Longrightarrow> x \<in> \<lbrakk>G1\<rbrakk>"
-    by (unfold transformStart_def NonTerminals_def NTInRule_def Lang_def Language_def Produces_def IsTerminalWord_def, auto, simp add: Start_Part2)
+    by (metis Start_Part2 transformStart_def)
   from 1 and 2 show ?thesis
     by blast
 qed
@@ -95,134 +615,399 @@ definition transformTermSingle :: "('n, 't) CFG \<Rightarrow> 'n \<Rightarrow> (
                                  \<and> R1 = (S1, L @ (T(a) # R))
                                  \<and> R2 = (S1, L @ (NT(N) # R))
                                  \<and> R3 = (N, [T a])
+                                 \<and> (L @ R \<noteq> [])
                                  \<and> (S, Rs2) = G2 
+                                 \<and> R1 \<in> Rs1
                                  \<and> Rs2 = {R2, R3} \<union> (Rs1 - {R1})
                                  \<and> NT(N) \<notin> NonTerminals(G1)"
 
-lemma Term_Part1:
-  assumes a: "R1 = (S1, L @ T a # R)"
-  assumes b: "R2 = (S1, L @ NT N # R)"
-  assumes c: "R3 = (N, [T a])"
-  assumes d: "G1 = (S, Rs1)"
-  assumes e: "G2 = (S, Rs2)"
-  assumes f: "IsTerminalWord x"
-  assumes g: "[NT S] -Rs1\<rightarrow>\<^sup>n x"
-  assumes h: "Rs2 = {R2, R3} \<union> (Rs1 - {R1})"
-  assumes i: "NT N \<notin> NonTerminals G1"
-  shows      "\<exists>n. [NT S] -Rs2\<rightarrow>\<^sup>n x"
-  using a and b and c and d and e and f and g and h and i apply-
-  apply(induction n, auto, simp add: IsTerminalWord_def)
-  done
+lemma Term_Part1_induct1:
+  assumes p: "transformTermSingle G1 N G2"
+  assumes g: "(NT N) \<notin> set A"
+  assumes l: "\<And>A x. ((NT N) \<notin> set A \<and> A -(snd G1)\<rightarrow>\<^sup>n x \<Longrightarrow> A -(snd G2)\<rightarrow>\<^sup>* x)"
+  assumes m: "ProducesInN A (snd G1) (Suc n) x"
+  shows      "A -(snd G2)\<rightarrow>\<^sup>* x"
+proof-
+  from p have q: "\<exists> S R1 R2 R3 Rs1 Rs2 S1 L R a. 
+                  (S, Rs1) = G1 
+                  \<and> R1 = (S1, L @ (T(a) # R))
+                  \<and> R2 = (S1, L @ (NT(N) # R))
+                  \<and> R3 = (N, [T a])
+                  \<and> (L @ R \<noteq> [])
+                  \<and> (S, Rs2) = G2 
+                  \<and> R1 \<in> Rs1
+                  \<and> Rs2 = {R2, R3} \<union> (Rs1 - {R1})
+                  \<and> NT(N) \<notin> NonTerminals(G1)"
+          (is "\<exists> S R1 R2 R3 Rs1 Rs2 S1 L R a. ?P S R1 R2 R3 Rs1 Rs2 S1 L R a")
+    by (simp add: transformTermSingle_def)
+  then obtain S R1 R2 R3 Rs1 Rs2 S1 L R a where r: "?P S R1 R2 R3 Rs1 Rs2 S1 L R a" by blast
+  from r have a: "R1 = (S1, L @ T a # R)" by auto
+  from r have b: "R2 = (S1, L @ NT N # R)" by auto
+  from r have c: "R3 = (N, [T a])" by auto
+  from r have d: "(L @ R \<noteq> [])" by auto
+  from r have e: "G1 = (S, Rs1)" by auto
+  from r have f: "G2 = (S, Rs2)" by auto
+  from r have i: "R1 \<in> Rs1" by auto
+  from r have j: "Rs2 = {R2, R3} \<union> (Rs1 - {R1})" by auto
+  from r have k: "NT N \<notin> NonTerminals G1" by auto
+  from m and e have 0: "\<exists> t. A -Rs1\<rightarrow> t \<and> t -Rs1\<rightarrow>\<^sup>n x" (is "\<exists> t. ?P t")
+    by simp
+  then obtain t where 1: "?P t" by blast
+  from j have 00: "\<And> T. T \<in> Rs1 \<Longrightarrow> T = R1 \<or> T \<in> Rs2"
+    by blast
+  from a and 00 have 2: "\<And> A B. (A, B) \<in> Rs1 \<Longrightarrow> (A = S1 \<and> B = L @ T a # R) \<or> (A, B) \<in> Rs2"
+    by blast
+  show ?thesis
+proof cases
+  assume x: "\<exists> l r. A = l @ [NT S1] @ r \<and> t = l @ L @ T a # R @ r" (is "\<exists> l r. ?P l r")
+  then obtain l r where 3: "?P l r" by blast
+  from b and j and x and 3 have 4: "A -Rs2\<rightarrow> l @ L @ NT N # R @ r"
+    apply(unfold ProductionStep_def Productions_def)
+    by (smt (verit, ccfv_threshold) Cons_eq_appendI Un_commute Un_insert_right append_assoc insert_iff mem_Collect_eq)
+  from c and j and x have 5: "(N, [T a]) \<in> Rs2"
+    by blast
+  from 5 and 3 have 6: "l @ L @ NT N # R @ r -Rs2\<rightarrow> t"
+    apply(unfold ProductionStep_def Productions_def) 
+    by (smt (verit, del_insts) Cons_eq_appendI append_Nil append_assoc mem_Collect_eq)
+  from 6 and 4 have 7: "A -Rs2\<rightarrow>\<^sup>* t" 
+    by (meson ProducesInN.simps(1) ProducesInN.simps(2) Produces_def)
+  from k and a and i have 8: "(NT N) \<notin> set (L @ T a # R)"
+    apply(unfold NonTerminals_def)
+    using NTInRule_def e by fastforce
+  from g and 3 have 9: "(NT N) \<notin> set l \<and> (NT N) \<notin> set r"
+    by simp
+  from 8 and 9 and 3 have 10: "(NT N) \<notin> set t"
+    by simp
+  from 10 and l and 7 and 1 and e and f transitiveProductions show ?thesis  
+    by (metis snd_conv)
+next
+  assume y: "\<not> (\<exists> l r. A = l @ [NT S1] @ r \<and> t = l @ L @ T a # R @ r)"
+  from 1 have 3: "\<exists> l r P Rhs. A =  l @ [NT P] @ r \<and> t = l @ Rhs @ r \<and> (P, Rhs) \<in> Rs1" (is "\<exists>  l r P Rhs. ?P l r P Rhs")
+    by (smt (verit, ccfv_SIG) Pair_inject ProductionStep_def Productions_def mem_Collect_eq)
+  then obtain l r P Rhs where 4: "?P l r P Rhs" by blast
+  from 2 and 4 and y have 5: "(P, Rhs) \<in> Rs2"
+    by fastforce
+  from 5 have 6: "A -Rs2\<rightarrow> t" 
+    using "4" CollectI ProductionStep_def Productions_def by fastforce
+  from k and a and i and 3 have 8: "(NT N) \<notin> set Rhs"
+    apply(unfold NonTerminals_def)
+    using "4" NTInRule_def e by force
+  from g and 4 have 9: "(NT N) \<notin> set l \<and> (NT N) \<notin> set r"
+    by simp
+  from 8 and 9 and 4 have 10: "(NT N) \<notin> set t"
+    by simp
+  from 6 have 11: "A -Rs2\<rightarrow>\<^sup>* t" 
+    by (meson ProducesInN.simps(1) ProducesInN.simps(2) Produces_def)
+  from 1 and 10 and l and 11 and e and f and transitiveProductions show ?thesis
+    by fastforce
+  qed  
+qed
+
+lemma Term_Part1_induct2:
+  fixes      A :: "('n, 't) Elem list"
+  fixes      G1 :: "('n, 't) CFG"
+  assumes p: "transformTermSingle G1 N G2"
+  assumes l: "(NT N) \<notin> set A" 
+  assumes m: "A -(snd G1)\<rightarrow>\<^sup>n x"
+  shows      "A -(snd G2)\<rightarrow>\<^sup>* x"
+proof-
+  from p and l and Term_Part1_induct1 have 0: "\<And>A x. (NT N \<notin> set A \<and> A -snd G1\<rightarrow>\<^sup>n x \<Longrightarrow> A -snd G2\<rightarrow>\<^sup>* x)"
+    apply (induction n)
+    apply (metis ProducesInN.simps(1) Produces_def)
+    by (smt (verit) Term_Part1_induct1)
+  from 0 and m and l show ?thesis
+    by blast
+qed
   
+lemma Term_Part1:
+  assumes a: "transformTermSingle G1 N G2"
+  assumes b: "x \<in> \<lbrakk>G1\<rbrakk>"
+  shows      "x \<in> \<lbrakk>G2\<rbrakk>"
+proof-
+  from b have 0: "\<exists> n S Rs1. [NT S] -Rs1\<rightarrow>\<^sup>n x \<and> (S, Rs1) = G1" (is "\<exists> n S Rs1. ?P n S Rs1")
+    by (simp add: Language_def Lang_def Produces_def PartialEvalLanguage_def, auto)
+  then obtain n S Rs1 where 1: "?P n S Rs1" by blast
+  from Term_Part1_induct2 and a have 2: "\<And>A B x n. ((NT N) \<notin> set A \<and> A -(snd G1)\<rightarrow>\<^sup>n x \<Longrightarrow> A -(snd G2)\<rightarrow>\<^sup>* x)"
+    by metis
+  from a have 3: "NT N \<notin> NonTerminals G1"
+    by(unfold transformTermSingle_def, auto)
+  from 1 and 3 have 4: "N \<noteq> S"
+    by(unfold NonTerminals_def, auto)
+  from 4 have 5: "NT N \<notin> set ([NT S])"
+    by simp
+  from 5 and 2 and 1 have 6: "[NT S] -(snd G2)\<rightarrow>\<^sup>* x"
+    by force
+  from a and 1 have 7: "\<exists> Rs2. G2 = (S, Rs2)" (is "\<exists> Rs2. ?P Rs2")
+    by(unfold transformTermSingle_def, blast)
+  then obtain Rs2 where 8: "?P Rs2" by blast
+  from b have 9: "IsTerminalWord x" 
+    by (unfold Lang_def Language_def PartialEvalLanguage_def, auto)
+  from 8 and 6 and 9 show ?thesis
+    by (unfold Lang_def Language_def PartialEvalLanguage_def, auto)
+qed
+
+
+lemma Term_Part2_induct1:
+  assumes a: "transformTermSingle G1 N G2"
+  assumes b: "(NT N) \<notin> set A"
+  assumes c: "\<And>m A x. (m \<le> n \<and> IsTerminalWord x \<and> (NT N) \<notin> set A \<and> A -(snd G2)\<rightarrow>\<^sup>m x \<Longrightarrow> A -(snd G1)\<rightarrow>\<^sup>* x)"
+  assumes d: "ProducesInN A (snd G2) (Suc n) x"
+  assumes p: "IsTerminalWord x"
+  shows      "A -(snd G1)\<rightarrow>\<^sup>* x"
+proof-
+  from a have 0: "\<exists> S R1 R2 R3 Rs1 Rs2 S1 L R a. 
+                  (S, Rs1) = G1 
+                  \<and> R1 = (S1, L @ (T(a) # R))
+                  \<and> R2 = (S1, L @ (NT(N) # R))
+                  \<and> R3 = (N, [T a])
+                  \<and> (L @ R \<noteq> [])
+                  \<and> (S, Rs2) = G2 
+                  \<and> R1 \<in> Rs1
+                  \<and> Rs2 = {R2, R3} \<union> (Rs1 - {R1})
+                  \<and> NT(N) \<notin> NonTerminals(G1)"
+          (is "\<exists> S R1 R2 R3 Rs1 Rs2 S1 L R a. ?P S R1 R2 R3 Rs1 Rs2 S1 L R a")
+    by (simp add: transformTermSingle_def)
+  then obtain S R1 R2 R3 Rs1 Rs2 S1 L R a where 1: "?P S R1 R2 R3 Rs1 Rs2 S1 L R a" by blast
+  from 1 have e: "R1 = (S1, L @ T a # R)" by auto
+  from 1 have f: "R2 = (S1, L @ NT N # R)" by auto
+  from 1 have g: "R3 = (N, [T a])" by auto
+  from 1 have h: "(L @ R \<noteq> [])" by auto
+  from 1 have i: "G1 = (S, Rs1)" by auto
+  from 1 have j: "G2 = (S, Rs2)" by auto
+  from 1 have k: "R1 \<in> Rs1" by auto
+  from 1 have l: "Rs2 = {R2, R3} \<union> (Rs1 - {R1})" by auto
+  from 1 have m: "NT N \<notin> NonTerminals G1" by auto
+  from d and j have 0: "\<exists> t. A -Rs2\<rightarrow> t \<and> t -Rs2\<rightarrow>\<^sup>n x" (is "\<exists> t. ?P t")
+    by simp
+  then obtain t where 2: "?P t" by blast
+  from l have 3: "\<And> T. T \<in> Rs2 \<Longrightarrow> (T = R2 \<or> T = R3) \<or> T \<in> Rs1" (* r2 is fine, r3 isn't *)
+    by blast
+  from f have 4: "(NT N) \<in> (set (snd R2))"
+    by auto
+  from 2 have 5: "\<exists> l r rhs N'. A = l @ [NT N'] @ r \<and> t = l @ rhs @ r \<and> (N', rhs) \<in> Rs2"
+    (is "\<exists> l r rhs N'. ?P l r rhs N'")
+    by (unfold ProductionStep_def Productions_def, auto) 
+  then obtain l r rhs N' where 6: "?P l r rhs N'" by blast
+  from 3 and 6 have 7: "(N', rhs) = R2 \<or> (N', rhs) = R3 \<or> (N', rhs) \<in> Rs1"
+    by auto
+  from 6 and g and 3 and b have 8: "(N', rhs) \<noteq> R3" 
+    by auto
+  from 8 and 7 have 9: "(N', rhs) = R2 \<or> (N', rhs) \<in> Rs1"
+    by auto
+  then show ?thesis
+proof 
+  assume x: "(N', rhs) = R2"
+  from f and x and 6 have 10: "t = l @ L @ [NT N] @ R @ r" by auto
+  from 10 and 2 and p and OrderInvStep have 11: "\<exists>rhs1. (N, rhs1) \<in> Rs2 \<and> ProducesInN (l @ L @ rhs1 @ R @ r) Rs2 (n-1) x"
+    (is "\<exists> rhs1. ?P rhs1")
+    by (metis append.assoc)
+  then obtain rhs1 where 12: "?P rhs1" by blast
+  from m and i have 13: "\<And> rhs. (N, rhs) \<notin> Rs1"
+    by(unfold NonTerminals_def NTInRule_def, blast)
+  from 3 and 12 and 13 and f and g have 14: "(N, rhs1) = R3"
+    using "1" by blast
+  from 14 and g have 15: "rhs1 = [T a]" by auto
+  from m and k and e have 16: "(NT N) \<notin> set L \<and> (NT N) \<notin> set R"
+    by (smt (verit, ccfv_threshold) "1" NTInRule_def NonTerminals_def Un_iff insert_iff list.simps(15) mem_Collect_eq set_append)
+  from b and 6 have 17: "(NT N) \<notin> set l \<and> (NT N) \<notin> set r"
+    by simp
+  from 16 and 17 and 15 have 18: "(NT N) \<notin> set (l @ L @ rhs1 @ R @ r)"
+    by simp
+  from c and 18 and 12 have 19: "(l @ L @ rhs1 @ R @ r) -Rs1\<rightarrow>\<^sup>* x"
+    by (metis "1" diff_le_self p snd_conv)
+  from e and k have 20: "l @ [NT S1] @ r -Rs1\<rightarrow> l @ L @ [T a] @ R @ r"
+    apply(unfold ProductionStep_def Productions_def)
+    by fastforce
+  from x and 6 and 15 and 20 and f have 21: "A -Rs1\<rightarrow> l @ L @ rhs1 @ R @ r"
+    by force
+  from 21 and 19 show ?thesis
+    by (metis ProducesInN.simps(2) Produces_def i snd_conv)
+next
+  assume x: "(N', rhs) \<in> Rs1"
+  from x and 6 have 10: "A -Rs1\<rightarrow> t"
+    apply(unfold ProductionStep_def Productions_def)
+    by blast
+  from m and k and e have 11: "(NT N) \<notin> set L \<and> (NT N) \<notin> set R"
+    by (smt (verit, ccfv_threshold) "1" NTInRule_def NonTerminals_def Un_iff insert_iff list.simps(15) mem_Collect_eq set_append)
+  from b and 6 have 12: "(NT N) \<notin> set l \<and> (NT N) \<notin> set r"
+    by simp
+  from x and m have 13: "(NT N) \<notin> set rhs"
+    by (smt (verit) "1" CollectI NTInRule_def NonTerminals_def)
+  from 13 and 12 and 6 have 14: "(NT N) \<notin> set t"
+    by auto
+  from 14 and 2 and c have 15: "t -Rs1\<rightarrow>\<^sup>* x"
+    using i j p by auto
+  from 15 and 10 show ?thesis
+    by (metis ProducesInN.simps(2) Produces_def i snd_eqD)
+  qed
+qed
+
+lemma Term_Part2_induct2:
+  assumes a: "transformTermSingle G1 N G2"
+  assumes b: "(NT N) \<notin> set A"
+  assumes c: "\<And>m A x. (m < n \<and> IsTerminalWord x \<and> (NT N) \<notin> set A \<and> A -(snd G2)\<rightarrow>\<^sup>m x \<Longrightarrow> A -(snd G1)\<rightarrow>\<^sup>* x)"
+  assumes d: "ProducesInN A (snd G2) n x"
+  assumes p: "IsTerminalWord x"
+  shows      "A -(snd G1)\<rightarrow>\<^sup>* x"
+proof-
+  have "n > 0 \<or> n = 0" by auto
+  then show ?thesis
+  proof
+    assume x: "n > 0"
+    from x have 0: "\<exists> n'. n' = n-1" (is "\<exists> n'. ?P n'") by auto
+    then obtain n' where 1: "?P n'" by blast
+    from 1 and c have 2: "\<And>m A x. (m \<le> n' \<and> IsTerminalWord x \<and> (NT N) \<notin> set A \<and> A -(snd G2)\<rightarrow>\<^sup>m x \<Longrightarrow> A -(snd G1)\<rightarrow>\<^sup>* x)"
+      by (metis Suc_pred' less_Suc_eq_le x)
+    from 1 and d have 3: "ProducesInN A (snd G2) (Suc n') x"
+      by (simp add: x)
+    from 2 and 3 and p and a and b and Term_Part2_induct1 show ?thesis
+      by (metis (no_types, lifting))      
+  next
+    assume y: "n = 0"
+    from d and y have 0: "x = A"
+      by simp
+    from 0 show ?thesis
+      by (meson ProducesInN.simps(1) Produces_def)
+  qed
+qed
+
+lemma Term_Part2_induct3:
+  fixes      A :: "('n, 't) Elem list"
+  fixes      G1 :: "('n, 't) CFG"
+  assumes p: "transformTermSingle G1 N G2"
+  assumes l: "(NT N) \<notin> set A" 
+  assumes k: "IsTerminalWord x"
+  assumes m: "A -(snd G2)\<rightarrow>\<^sup>n x"
+  shows      "A -(snd G1)\<rightarrow>\<^sup>* x"
+proof-
+  have 0: "\<And>A x. IsTerminalWord x \<and> (NT N) \<notin> set A \<and> A -(snd G2)\<rightarrow>\<^sup>n x \<Longrightarrow> A -(snd G1)\<rightarrow>\<^sup>* x"
+    apply (induction n rule: less_induct)
+    by (smt (verit, best) Term_Part2_induct2 p)
+  from 0 and p and l and m and k show ?thesis 
+    by simp
+qed
+
 lemma Term_Part2:
-  assumes a: "R1 = (S1, L @ T a # R)"
-  assumes b: "R2 = (S1, L @ NT N # R)"
-  assumes c: "R3 = (N, [T a])"
-  assumes d: "G1 = (S, Rs1)"
-  assumes e: "G2 = (S, Rs2)"
-  assumes f: "IsTerminalWord x"
-  assumes g: "[NT S] -Rs2\<rightarrow>\<^sup>n x"
-  assumes h: "Rs2 = {R2, R3} \<union> (Rs1 - {R1})"
-  assumes i: "NT N \<notin> NonTerminals G1"
-  shows      "\<exists>n. [NT S] -Rs1\<rightarrow>\<^sup>n x"
-  using a and b and c and d and e and f and g and h and i apply-
-  apply(induction n, auto, simp add: IsTerminalWord_def)
-  done
+  assumes a: "transformTermSingle G1 N G2"
+  assumes b: "x \<in> \<lbrakk>G2\<rbrakk>"
+  shows      "x \<in> \<lbrakk>G1\<rbrakk>"
+proof-
+  from b have 0: "\<exists> n S Rs2. [NT S] -Rs2\<rightarrow>\<^sup>n x \<and> (S, Rs2) = G2" (is "\<exists> n S Rs2. ?P n S Rs2")
+    by (simp add: Language_def Lang_def Produces_def PartialEvalLanguage_def, auto)
+  then obtain n S Rs2 where 1: "?P n S Rs2" by blast
+  from Term_Part2_induct3 and a have 2: "\<And>A B x n. ((NT N) \<notin> set A \<and> IsTerminalWord x \<and> A -(snd G2)\<rightarrow>\<^sup>n x \<Longrightarrow> A -(snd G1)\<rightarrow>\<^sup>* x)"
+    by metis
+  from a have 3: "NT N \<notin> NonTerminals G1"
+    by(unfold transformTermSingle_def, auto)
+  from a and 1 and 3 have 4: "N \<noteq> S"
+    by (unfold NonTerminals_def transformTermSingle_def, auto)
+  from 4 have 5: "NT N \<notin> set ([NT S])"
+    by simp
+  from b have 6: "IsTerminalWord x"
+    by (simp add: Lang_def Language_def PartialEvalLanguage_def)
+  from 5 and 2 and 1 and 6 have 7: "[NT S] -(snd G1)\<rightarrow>\<^sup>* x"
+    by force
+  from a and 1 have 8: "\<exists> Rs1. G1 = (S, Rs1)" (is "\<exists> Rs1. ?P Rs1")
+    by(unfold transformTermSingle_def, auto)
+  then obtain Rs1 where 9: "?P Rs1" by blast
+  from 9 and 7 and 6 show ?thesis
+    by(unfold Lang_def Language_def PartialEvalLanguage_def, auto)
+qed
 
 theorem verifyTransformTerm: 
   assumes a: "transformTermSingle G1 N G2"
   shows      "\<lbrakk>G1\<rbrakk> = \<lbrakk>G2\<rbrakk>"
 proof-
-  from a have 0: "\<exists> S R1 R2 R3 Rs1 Rs2 S1 L R a. 
-                    (S, Rs1) = G1 
-                    \<and> R1 = (S1, L @ (T(a) # R))
-                    \<and> R2 = (S1, L @ (NT(N) # R))
-                    \<and> R3 = (N, [T a])
-                    \<and> (S, Rs2) = G2 
-                    \<and> Rs2 = {R2, R3} \<union> (Rs1 - {R1})
-                    \<and> NT(N) \<notin> NonTerminals(G1)" 
-                  (is "\<exists>S R1 R2 R3 Rs1 Rs2 S1 L R a. ?P S R1 R2 R3 Rs1 Rs2 S1 L R a")
-    by (simp add: transformTermSingle_def)
-  from 0 obtain S R1 R2 R3 Rs1 Rs2 S1 L R a where 1: "?P S R1 R2 R3 Rs1 Rs2 S1 L R a" by blast
-  from 1 have 2: "\<And>x. x \<in> \<lbrakk>G1\<rbrakk> \<Longrightarrow> x \<in> \<lbrakk>G2\<rbrakk>"
-    by (unfold Lang_def Language_def Produces_def, auto, simp add: Term_Part1)
-  from 1 have 3: "\<And>x. x \<in> \<lbrakk>G2\<rbrakk> \<Longrightarrow> x \<in> \<lbrakk>G1\<rbrakk>"
-    by (unfold Lang_def Language_def Produces_def, auto, simp add: Term_Part2)
-  from 2 and 3 show ?thesis
-    using "1" by fastforce
+  from a have 0: "\<And>x. x \<in> \<lbrakk>G1\<rbrakk> \<Longrightarrow> x \<in> \<lbrakk>G2\<rbrakk>"
+    by (simp add: Term_Part1)
+  from a have 1: "\<And>x. x \<in> \<lbrakk>G2\<rbrakk> \<Longrightarrow> x \<in> \<lbrakk>G1\<rbrakk>"
+    by (simp add: Term_Part2)
+  from 0 and 1 show ?thesis
+    by fastforce
 qed
-
 
 definition transformBinSingle :: "('n, 't) CFG \<Rightarrow> 'n \<Rightarrow> ('n, 't) CFG \<Rightarrow> bool"
-  where "transformBinSingle G1 N G2 \<equiv> \<exists> S R1 R2 R3 Rs1 Rs2 S1 a b c. 
+  where "transformBinSingle G1 N G2 \<equiv> \<exists> S R1 R2 R3 Rs1 Rs2 S1 L R a. 
                                    (S, Rs1) = G1 
+                                 \<and> R1 = (S1, L @ a # R)
+                                 \<and> R2 = (S1, L @ [NT N])
+                                 \<and> R3 = (N, a # R)  
+                                 \<and> L \<noteq> [] \<and> R \<noteq> []
                                  \<and> (S, Rs2) = G2 
+                                 \<and> R1 \<in> Rs1
                                  \<and> Rs2 = {R2, R3} \<union> (Rs1 - {R1})
-                                 \<and> NT(N) \<notin> NonTerminals(G1)
-                                 \<and> R1 = (S1, a # b # c)
-                                 \<and> R2 = (S1, a # [NT N])
-                                 \<and> R3 = (N, b # c)"
+                                 \<and> NT(N) \<notin> NonTerminals(G1)"
 
-lemma Bin_Part1:
-  assumes a: "R1 = (S1, a # b # c)"
-  assumes b: "R2 = (S1, [a, NT N])"
-  assumes c: "R3 = (N, b # c)"
-  assumes d: "G1 = (S, Rs1)"
-  assumes e: "G2 = (S, Rs2)"
-  assumes f: "IsTerminalWord x"
-  assumes g: "x \<in> \<lbrakk>G1\<rbrakk>"
-  assumes h: "Rs2 = {R2, R3} \<union> (Rs1 - {R1})"
-  assumes i: "NT N \<notin> NonTerminals G1"
-  shows      "x \<in> \<lbrakk>G2\<rbrakk>"
+lemma Bin_Part1_induct1:
+  assumes p: "transformBinSingle G1 N G2"
+  assumes g: "(NT N) \<notin> set A"
+  assumes l: "\<And>A x. ((NT N) \<notin> set A \<and> A -(snd G1)\<rightarrow>\<^sup>n x \<Longrightarrow> A -(snd G2)\<rightarrow>\<^sup>* x)"
+  assumes m: "ProducesInN A (snd G1) (Suc n) x"
+  shows      "A -(snd G2)\<rightarrow>\<^sup>* x"
 proof-
-  from g and d have 0: "\<exists> n. [NT S] -Rs1\<rightarrow>\<^sup>n x" (is "\<exists> n. ?P n")
-    by (unfold Lang_def Language_def Produces_def, auto)
-  then obtain n where 1: "?P n" by blast
-  from a and b and c and d and e and f and h and 1 show ?thesis
-  by(induction n, simp add: IsTerminalWord_def, auto)
-qed
-
-lemma Bin_Part2:
-  assumes a: "R1 = (S1, a # b # c)"
-  assumes b: "R2 = (S1, [a, NT N])"
-  assumes c: "R3 = (N, b # c)"
-  assumes d: "G1 = (S, Rs1)"
-  assumes e: "G2 = (S, Rs2)"
-  assumes f: "IsTerminalWord x"
-  assumes g: "x \<in> \<lbrakk>G2\<rbrakk>"
-  assumes h: "Rs2 = {R2, R3} \<union> (Rs1 - {R1})"
-  assumes i: "NT N \<notin> NonTerminals G1"
-  shows      "x \<in> \<lbrakk>G1\<rbrakk>"
-proof-
-  from g and e have 0: "\<exists> n. [NT S] -Rs2\<rightarrow>\<^sup>n x" (is "\<exists> n. ?P n")
-    by (unfold Lang_def Language_def Produces_def, auto)
-  then obtain n where 1: "?P n" by blast
-  from a and b and c and d and e and f and h and 1 show ?thesis
-  by(induction n, simp add: IsTerminalWord_def, auto)
-qed
-
-theorem verifyTransformBin: 
-  assumes a: "transformBinSingle G1 N G2"
-  shows      "\<lbrakk>G1\<rbrakk> = \<lbrakk>G2\<rbrakk>"
-proof-
-  from a have 0: "\<exists>S R1 R2 R3 Rs1 Rs2 S1 a b c. 
-                    (S, Rs1) = G1 
-                    \<and> (S, Rs2) = G2 
-                    \<and> Rs2 = {R2, R3} \<union> (Rs1 - {R1})
-                    \<and> NT(N) \<notin> NonTerminals(G1)
-                    \<and> R1 = (S1, a # b # c)
-                    \<and> R2 = (S1, a # [NT N])
-                    \<and> R3 = (N, b # c)" 
-                  (is "\<exists>S R1 R2 R3 Rs1 Rs2 S1 a b c. ?P S R1 R2 R3 Rs1 Rs2 S1 a b c")
+  from p have q: "\<exists> S R1 R2 R3 Rs1 Rs2 S1 L R a. 
+                  (S, Rs1) = G1 
+                  \<and> R1 = (S1, L @ a # R)
+                  \<and> R2 = (S1, L @ [NT N])
+                  \<and> R3 = (N, a # R)  
+                  \<and> L \<noteq> [] \<and> R \<noteq> []
+                  \<and> (S, Rs2) = G2 
+                  \<and> R1 \<in> Rs1
+                  \<and> Rs2 = {R2, R3} \<union> (Rs1 - {R1})
+                  \<and> NT(N) \<notin> NonTerminals(G1)"
+          (is "\<exists> S R1 R2 R3 Rs1 Rs2 S1 L R a. ?P S R1 R2 R3 Rs1 Rs2 S1 L R a")
     by (simp add: transformBinSingle_def)
-  from 0 obtain S R1 R2 R3 Rs1 Rs2 S1 a b c where 1: "?P S R1 R2 R3 Rs1 Rs2 S1 a b c" by blast
-  from 1 have 2: "\<And>x. x \<in> \<lbrakk>G1\<rbrakk> \<Longrightarrow> x \<in> \<lbrakk>G2\<rbrakk>"
-    by (smt (verit) Bin_Part1 Lang_def Language_def mem_Collect_eq)
-  from 1 have 3: "\<And>x. x \<in> \<lbrakk>G2\<rbrakk> \<Longrightarrow> x \<in> \<lbrakk>G1\<rbrakk>"
-    by (smt (verit) Bin_Part2 Lang_def Language_def mem_Collect_eq)
-  from 2 and 3 show ?thesis
+  then obtain S R1 R2 R3 Rs1 Rs2 S1 L R a where r: "?P S R1 R2 R3 Rs1 Rs2 S1 L R a" by blast
+  from r have a: "R1 = (S1, L @ a # R)" by auto
+  from r have b: "R2 = (S1, L @ [NT N])" by auto
+  from r have c: "R3 = (N, a # R)" by auto
+  from r have d: "L \<noteq> [] \<and> R \<noteq> []" by auto
+  from r have e: "G1 = (S, Rs1)" by auto
+  from r have f: "G2 = (S, Rs2)" by auto
+  from r have i: "R1 \<in> Rs1" by auto
+  from r have j: "Rs2 = {R2, R3} \<union> (Rs1 - {R1})" by auto
+  from r have k: "NT N \<notin> NonTerminals G1" by auto
+  from m and e have 0: "\<exists> t. A -Rs1\<rightarrow> t \<and> t -Rs1\<rightarrow>\<^sup>n x" (is "\<exists> t. ?P t")
+    by simp
+  then obtain t where 1: "?P t" by blast
+  from j have 00: "\<And> T. T \<in> Rs1 \<Longrightarrow> T = R1 \<or> T \<in> Rs2"
     by blast
+  from a and 00 have 2: "\<And> A B. (A, B) \<in> Rs1 \<Longrightarrow> (A = S1 \<and> B = L @ a # R) \<or> (A, B) \<in> Rs2"
+    by blast
+  from 1 have 3: "\<exists> l r rhs N'. A = l @ [NT N'] @ r \<and> t = l @ rhs @ r \<and> (N', rhs) \<in> Rs1"
+    (is "\<exists> l r rhs N'. ?P l r rhs N'")
+    by (unfold ProductionStep_def Productions_def, auto) 
+  then obtain l r rhs N' where 4: "?P l r rhs N'" by blast
+  from k and 4 and e have 10: "NT N \<notin> set rhs"
+    using NTInRule_def NonTerminals_def by force
+  from 10 and g and 4 have 11: "NT N \<notin> set t"
+    by simp
+  from 2 and 4 have 5: "(N' = S1 \<and> rhs = L @ a # R) \<or> (N', rhs) \<in> Rs2"
+    by auto
+  then show ?thesis
+  proof 
+    assume x: "(N' = S1 \<and> rhs = L @ a # R)"
+    from c have 6: "L @ [NT N] -Rs2\<rightarrow> L @ a # R"
+      apply (unfold ProductionStep_def Productions_def)
+      using r by fastforce
+    from b have 7: "[NT S1] -Rs2\<rightarrow> L @ [NT N]"
+      apply (unfold ProductionStep_def Productions_def)
+      using r by fastforce
+    from 6 and 7 have 8: "[NT S1] -Rs2\<rightarrow>\<^sup>* L @ a # R"
+      by (meson ProducesInN.simps(1) ProducesInN.simps(2) Produces_def)
+    from 8 have 9: "A -Rs2\<rightarrow>\<^sup>* t"
+      using "4" productionAppend3 x by blast
+    from 9 and 1 and l and 11 show ?thesis
+      using e f transitiveProductions by fastforce
+  next
+    assume y: "(N', rhs) \<in> Rs2"
+    from y and 4 have 6: "A -Rs2\<rightarrow> t"
+      using ProductionStep_def Productions_def by fastforce
+    from 6 and 1 and l and 11 show ?thesis
+      by (metis ProducesInN.simps(2) Produces_def e f snd_conv)
+  qed
 qed
+    
 
 definition DelNTFromRuleSet :: "'n \<Rightarrow> (('n, 't) Rule \<times> ('n, 't) Rule) set"
   where "DelNTFromRuleSet N \<equiv> {((S, l @ r), (S, l @ NT(N) # r)) | S l r. True}\<^sup>*"
@@ -435,37 +1220,6 @@ proof-
   from 2 and 3 show ?thesis
     by blast
 qed
-(*
-type_synonym ('n, 't) Grammar = "'n \<times> ('n, 't) Rule list"
-definition convCFG :: "('n, 't) Grammar \<Rightarrow> ('n, 't) CFG"
-  where "convCFG G = (fst G, set (snd G))"
-
-definition transTerm :: "('n, 't) Grammar \<Rightarrow> 'n \<Rightarrow> ('n, 't) Grammar \<Rightarrow> bool"
-  where "transTerm G1 N G2 \<equiv> transformTermSingle (convCFG(G1)) N (convCFG(G2))" 
-
-fun TerminalCount :: "('n, 't) Elem list \<Rightarrow> nat"
-  where "TerminalCount Nil = 0" |
-        "TerminalCount (T(a) # R) = 1 + TerminalCount R" |
-        "TerminalCount (NT(a) # R) = TerminalCount R"
-
-fun TerminalCountNonSingle :: "('n, 't) Elem list \<Rightarrow> nat"
-  where "TerminalCountNonSingle ([T(a)]) = 0" |
-        "TerminalCountNonSingle R = TerminalCount R"
-
-fun MetricTerm1 :: "('n, 't) Rule list \<Rightarrow> nat"
-  where "MetricTerm1 Nil = 0" |
-        "MetricTerm1 ((_, R) # Rs) = (TerminalCountNonSingle R) + (MetricTerm1 Rs)"
-
-fun MetricTerm :: "('n, 't) Grammar \<Rightarrow> nat"
-  where "MetricTerm (S, R) = MetricTerm1 R"
-
-theorem TerminationStart :
-  assumes a: "transTerm G1 N G2"
-  shows      "MetricTerm G1 > MetricTerm G2"
-  using a apply-
-  apply(simp add: transTerm_def transformTermSingle_def convCFG_def)
-  sledgehammer  
-*)
 
 definition DelAllNullableNTsFromRules :: "('n, 't) RuleSet \<Rightarrow> ('n, 't) RuleSet"
   where "DelAllNullableNTsFromRules X = {R | R N. R \<in> DelNTFromRule N X \<and> Nil \<in> \<lbrakk>N\<rbrakk>\<^sub>X}"
@@ -531,7 +1285,7 @@ proof-
 qed
 
 definition finiteCFG :: "('n, 't) CFG \<Rightarrow> bool"
-  where "finiteCFG G \<equiv> \<exists> S R. (S, R) = G \<and> finite R"
+  where "finiteCFG G \<equiv> finite (snd G)"
 
 lemma StartFinite:
   assumes a: "transformStart G1 S0 G2"
@@ -539,7 +1293,7 @@ lemma StartFinite:
   shows      "finiteCFG G2"
 proof-
   from a and b show ?thesis
-    by (metis Pair_inject finiteCFG_def finite_insert transformStart_def)
+    by (metis finiteCFG_def finite_insert snd_conv transformStart_def)
 qed
 
 lemma TermFinite:
@@ -657,128 +1411,8 @@ lemma UnitFinite:
   shows      "finiteCFG G2"
 proof-
   from a and b and UnitFinit_part5 show ?thesis
-    by (smt (verit) List.finite_set Pair_inject finiteCFG_def finite_Diff finite_distinct_list set_append transformUnitSingle2_def)
+    by (metis finiteCFG_def finite_Diff finite_UnI snd_conv transformUnitSingle2_def)
 qed
-
-(*
-definition listSuffixSet :: "'a list \<Rightarrow> 'a list set"
-  where "listSuffixSet R = {r. \<exists> l. R = l @ r}"
-
-definition listPrefixSet :: "'a list \<Rightarrow> 'a list set"
-  where "listPrefixSet R = {l. \<exists> r. R = l @ r}"
-
-lemma listSuffixInduct:
-  fixes      Rhs :: "'a list"
-  shows      "listSuffixSet Rhs \<union> {a # Rhs} = listSuffixSet (a # Rhs) "
-  apply (unfold listSuffixSet_def, induct Rhs, auto)
-  apply (metis append_eq_Cons_conv append_is_Nil_conv)
-  apply (meson Cons_eq_append_conv)
-  done
-
-lemma listSuffixFinite:
-  fixes      Rhs :: "'a list"
-  shows      "finite (listSuffixSet Rhs)"
-  apply (unfold listSuffixSet_def, induct Rhs, auto)
-  apply (metis List.finite_set finite_Un list.set(1) list.simps(15) listSuffixInduct listSuffixSet_def)
-  done
-
-lemma listPrefixInduct:
-  fixes      Rhs :: "'a list"
-  shows      "(image (Cons a) (listPrefixSet Rhs)) \<union> {Nil} = listPrefixSet (a # Rhs)"
-  apply(unfold listPrefixSet_def, induction Rhs, auto)
-  apply (simp add: Cons_eq_append_conv)
-  apply (smt (verit, ccfv_threshold) Cons_eq_append_conv image_iff mem_Collect_eq)
-  done
-
-lemma listPrefixFinite:
-  fixes      Rhs :: "'a list"
-  shows      "finite (listPrefixSet Rhs)"
-proof-
-  from finiteImage have 0: "\<And>a Rhs.
-       finite (listPrefixSet Rhs) \<Longrightarrow>
-       finite ((image (Cons a) (listPrefixSet Rhs)) \<union> {Nil})"
-    by blast
-  from listPrefixInduct have 1: "\<And>a Rhs.
-       finite ((image (Cons a) (listPrefixSet Rhs)) \<union> {Nil}) \<Longrightarrow>
-       finite (listPrefixSet (a # Rhs))"
-    by metis
-  from 0 and 1 have 2: "\<And>a Rhs. finite (listPrefixSet Rhs) \<Longrightarrow> finite (listPrefixSet (a # Rhs))"
-    by metis
-  show ?thesis
-    by(induction Rhs, unfold listPrefixSet_def, auto, fold listPrefixSet_def, simp add: 2)
-qed
-
-lemma DelFinite_Part1:
-  fixes      Rhs :: "'a list"
-  fixes      N :: "'a"
-  fixes      S :: "('a list \<times> 'a list) set"
-  assumes a: "S = {(l, r) | l r. Rhs = l @ (N # r)}"
-  shows      "finite S"
-proof-
-  from a have 0: "S \<subseteq> CartesianProduct (listPrefixSet Rhs) (listSuffixSet Rhs)"
-    by (unfold CartesianProduct_def listPrefixSet_def listSuffixSet_def, auto)
-  from listPrefixFinite and listSuffixFinite and CartesianFinite and 0 show ?thesis
-    by (metis finite_subset)
-qed
-
-fun DelFiniteConv :: "'n \<Rightarrow> (('n, 't) Elem list \<times> ('n, 't) Elem list) \<Rightarrow> ('n, 't) Rule"
-  where "DelFiniteConv S (L, R) = (S, L @ R)"
-
-lemma DelFinite_Part2:
-  fixes      Rhs :: "('n, 't) Elem list"
-  fixes      N :: "'n"
-  fixes      S :: "'n"
-  assumes a: "F = {w. \<exists>l r. w = (S, l @ r) \<and> Rhs = l @ ((NT N) # r)}"
-  shows      "finite F"
-proof-
-  have 0: "\<And>x. x \<in> {(S, l @ r) |l r. Rhs = l @ NT N # r} \<Longrightarrow> 
-           x \<in> image (DelFiniteConv S) {(l, r). Rhs = l @ ((NT N) # r)}"
-    by force
-  have 1: "\<And>x. x \<in> image (DelFiniteConv S) {(l, r). Rhs = l @ ((NT N) # r)} \<Longrightarrow>
-           x \<in> {(S, l @ r) |l r. Rhs = l @ NT N # r}"
-    by fastforce
-  from 0 and 1 and a have 2: "F = image (DelFiniteConv S) {(l, r). Rhs = l @ ((NT N) # r)}"
-    by blast
-  have 3: "finite {(l, r). Rhs = l @ ((NT N) # r)}"
-    by(rule_tac N="(NT N)" in DelFinite_Part1, auto)
-  from 3 and 2 show ?thesis
-    by (simp add: finiteImage)
-qed
-
-fun DelFiniteConv2 :: "'n \<Rightarrow> ('n, 't) Elem list \<Rightarrow> ('n, 't) Rule \<Rightarrow> (('n, 't) Rule \<times> ('n, 't) Rule )"
-  where "DelFiniteConv2 S Rhs R = ((S, Rhs), R)"
-
-lemma DelFinite_Part3:
-  fixes      Rhs :: "('n, 't) Elem list"
-  fixes      N :: "'n"
-  fixes      S :: "'n"
-  assumes a: "F = {((S, Rhs), w) | l r w. w = (S, l @ r) \<and> Rhs = l @ ((NT N) # r)}"
-  shows      "finite F"
-proof-
-  from a have 0: "{((S, Rhs), w) | l r w. w = (S, l @ r) \<and> Rhs = l @ ((NT N) # r)} = image (DelFiniteConv2 S Rhs) 
-                  {w. \<exists>l r. w = (S, l @ r) \<and> Rhs = l @ ((NT N) # r)}"
-    by (auto)
-  from 0 show ?thesis
-    by (simp add: DelFinite_Part2 assms)
-qed
-
-
-
-
-fun nthTransitive :: "nat \<Rightarrow> ('a \<times> 'a) set \<Rightarrow> ('a \<times> 'a) set"
-  where "nthTransitive 0 S = {}" |
-        "nthTransitive (Suc N) S = {(a, b) | a b c. (a, b) \<in> S \<or> (a, c) \<in> S \<and> (b, c) \<in> (nthTransitive N S)}"
-
-lemma transitivityMonotonic:
-  fixes      L :: "('a \<times> 'a) set"
-  fixes      f :: "'a \<Rightarrow> nat"
-  assumes a: "\<And> A B. (A, B) \<in> L \<Longrightarrow> (f A) < (f B)"
-  assumes c: "(A, B) \<in> (L\<^sup>+)"
-  shows      "(f A) < (f B)"
-  using a and c apply-
-  apply(unfold trancl_def tranclp_def, auto)
-  sledgehammer
-*)
 
 lemma listFinite:
   fixes      L :: "'a list"
@@ -859,41 +1493,6 @@ proof-
     by (smt (verit, ccfv_SIG))
 qed  
 
-(*
-(?a, ?b) \<in> ?r\<^sup>+ \<Longrightarrow>
-    (\<And>y. (?a, y) \<in> ?r \<Longrightarrow> ?P y) \<Longrightarrow>
-    (\<And>y z. (?a, y) \<in> ?r\<^sup>+ \<Longrightarrow> (y, z) \<in> ?r \<Longrightarrow> ?P y \<Longrightarrow> ?P z) \<Longrightarrow> ?P ?b
-
-
-lemma MeasureTransitive :
-  fixes      L :: "('a \<times> 'a) set"
-  fixes      f :: "'a \<Rightarrow> nat"
-  assumes a: "L \<subseteq> (measure f)"
-  shows      "L\<^sup>+ \<subseteq> (measure f)"
-  sledgehammer
-*)
-
-(*
-lemma DelFinite_Part1:
-  fixes      H :: "(('n, 't) Rule \<times> ('n, 't) Rule) set" 
-  fixes      K :: "(('n, 't) Rule \<times> ('n, 't) Rule) set" 
-  assumes a: "H = {((S, l @ r), S, l @ NT N # r) | S l r. True}"
-  assumes b: "K = {((S, l @ r), S, l @ NT N # r) | S l r. True}\<^sup>+"
-  shows      "wf K"
-proof-
-  from a have 0: "\<And> A B. (A, B) \<in> H \<Longrightarrow> (RuleRhsSize A) < (RuleRhsSize B)"
-    by (unfold RuleRhsSize_def, force)
-  from 0 have 1: "H \<subseteq> (measure RuleRhsSize)"
-    by fastforce
-  from wf_measure have 2: "wf (measure RuleRhsSize)"
-    by auto
-  from 1 and 2 and wf_subset have 3: "wf H"
-    by blast
-  from 3 and wf_trancl show ?thesis
-    using a assms(2) by blast
-qed
-*)
-
 lemma DelFinite_Part5:
   fixes      Rhs :: "('n, 't) Elem list"
   fixes      N :: "'n"
@@ -907,15 +1506,6 @@ proof-
   from 0 and a show ?thesis
     by (unfold DelNTFromRuleSet_def, smt (verit, best) "0")
 qed
-
-(*
-lemma WellFoundedChainTermination:
-  fixes      L :: "('a \<times>'a) set"
-  assumes a: "wf L"
-  assumes b: "\<And> A. finite ({(B, A) | B. (B, A) \<in> L})"
-  shows      "\<And> A. finite ({(B, A) | B. (B, A) \<in> L\<^sup>+})"
-  sledgehammer
-*)
 
 lemma subsetListFinite:
   fixes      S :: "'a set"
@@ -1017,31 +1607,6 @@ proof-
     by (simp add: finite_subset)
 qed
 
-(*
-lemma DelFinite_Part4:
-  fixes      Rhs :: "('n, 't) Elem list"
-  fixes      N :: "'n"
-  fixes      S :: "'n"
-  assumes a: "H = {NR | NR. ((S, Rhs), NR) \<in> DelNTFromRuleSet N}"
-  shows      "(S, x) \<in> H \<Longrightarrow> (size x) < (size Rhs) \<or> (x = Rhs)"
-proof-
-  have 0:        "\<And>A B S. (A, B) \<in> S\<^sup>* \<Longrightarrow> A = B \<or> (A, B) \<in> S\<^sup>+"
-    by (meson rtranclD)
-  from 0 have 1: "\<And>S Rhs NR N. ((S, Rhs), NR) \<in> DelNTFromRuleSet N \<Longrightarrow> NR = (S, Rhs) 
-           \<or> ((S, Rhs), NR) \<in> {((S, l @ NT N # r), S, l @ r) | S l r. True}\<^sup>+"
-    by (unfold DelNTFromRuleSet_def, smt (verit) rtrancl_eq_or_trancl)
-  have 2: "\<And> l r a. (size (l @ a # r)) > (size (l @ r))"
-    by simp
-  from 2 have 3: "\<And> S Rhs1 Rhs2 N. 
-          ((S, Rhs1), (S, Rhs2)) \<in> {((S, l @ N # r), (S, l @ r)) | S l r. True} \<Longrightarrow>
-          (size Rhs2) < (size Rhs1)"
-    by force
-  from 3 have 4: "\<And> Rhs1 Rhs2 N. 
-          (Rhs1, Rhs2) \<in> {(l @ N # r, l @ r) | l r. True}\<^sup>+ \<Longrightarrow>
-          (size Rhs2) < (size Rhs1)"
-    sledgehammer
-*)
-
 lemma DelFinite_Part9:
   fixes      Rs1 :: "('n, 't) RuleSet"
   fixes      N :: "'n"
@@ -1113,9 +1678,112 @@ proof-
     by(unfold RemoveAllEpsilonProds_def, auto)
   from a and b and 0 show ?thesis
   apply (unfold transformDel2_def finiteCFG_def)
-    by (smt (verit, best) "0" DelFinite_Part11 finite_Un old.prod.inject sup.absorb_iff2)
+  using DelFinite_Part11 infinite_super by fastforce
 qed
 
+(* Measure for Term to prove that it terminates *)
 
+fun CountTerminals :: "('n, 't) Elem list \<Rightarrow> nat"
+  where "CountTerminals [] = 0" | 
+        "CountTerminals ((T a) # xs) = 1 + CountTerminals xs" | 
+        "CountTerminals ((NT a) # xs) = CountTerminals xs" 
 
+fun CountNonSingleTerminals :: "('n, 't) Rule \<Rightarrow> nat"
+  where "CountNonSingleTerminals (_, []) = 0" |
+        "CountNonSingleTerminals (_, a # []) = 0" | 
+        "CountNonSingleTerminals (_, El) = CountTerminals El"
+
+definition TermFold :: "('n, 't) Rule \<Rightarrow> nat \<Rightarrow> nat"
+  where "TermFold R N = N + (CountNonSingleTerminals R)"
+
+definition TermRuleMeasure :: "('n, 't) RuleSet \<Rightarrow> nat"
+  where "TermRuleMeasure R = Finite_Set.fold TermFold 0 R"
+
+definition TermMeasure :: "('n, 't) CFG \<Rightarrow> nat"
+  where "TermMeasure G = TermRuleMeasure (snd G)"
+
+lemma CountProperty1:
+  shows      "CountTerminals (L @ R) = CountTerminals L + CountTerminals R"
+  apply(induction L, auto)
+  by (smt (verit, best) CountTerminals.elims CountTerminals.simps(3) add.commute add_Suc_right list.distinct(1) list.sel(1) list.sel(3) plus_1_eq_Suc)
+
+lemma CountProperty2:
+  assumes a: "(L @ R \<noteq> [])"
+  shows      "CountNonSingleTerminals (S1, L @ (T(a) # R)) = CountNonSingleTerminals (S2, L @ (NT(N) # R)) + 1"
+proof-
+  from a have 0: "CountNonSingleTerminals (S1, L @ (T(a) # R)) = CountTerminals (L @ (T(a) # R))"
+    by (metis (no_types, opaque_lifting) CountNonSingleTerminals.simps(3) append_Cons append_Nil neq_Nil_conv)
+  from a have 1: "CountNonSingleTerminals (S2, L @ (NT(N) # R)) =  CountTerminals (L @ (NT(N) # R))"
+    by (metis (no_types, opaque_lifting) CountNonSingleTerminals.simps(3) append_Cons append_Nil neq_Nil_conv)
+  have 2: "CountTerminals (L @ (T(a) # R)) = CountTerminals (L @ (NT(N) # R)) + 1"
+    by (simp add: CountProperty1)
+  from 0 and 1 and 2 show ?thesis
+    by auto
+qed
+
+(*
+lemma foldInsert:
+  fixes      f :: "'a \<Rightarrow> 'b \<Rightarrow> 'b"
+  fixes      E :: "'a"
+  fixes      Z :: "'b"
+  assumes a: "comp_fun_commute_on (insert E S) f"
+  assumes b: "finite S"
+  assumes c: "E \<notin> S"
+  shows      "Finite_Set.fold f Z (insert E S) = f E (Finite_Set.fold f Z S)"
+proof-
+  from b have 0: "finite (insert E S)"
+    by blast
+  have 1: "S \<subseteq> (insert E S)"
+    by auto
+  from 0 and 1 and b and a and c and comp_fun_commute_on.fold_insert show ?thesis
+    apply (rule_tac S="(insert E S)" and f="f" and A="S" and x="E" and z="Z" in comp_fun_commute_on.fold_insert)
+    apply meson
+    apply force
+    apply blast
+    by blast
+qed
+*)
+
+lemma TermTerminate_Part1:
+  assumes a: "R1 = (S1, L @ T a # R)"
+  assumes b: "R2 = (S1, L @ NT N # R)"
+  assumes c: "R3 = (N, [T a])"
+  assumes d: "(L @ R \<noteq> [])"
+  assumes e: "G1 = (S, Rs1)"
+  assumes f: "G2 = (S, Rs2)"
+  assumes g: "R1 \<in> Rs1"
+  assumes h: "finite Rs1"
+  assumes i: "finite Rs2"
+  assumes j: "Rs2 = {R2, R3} \<union> (Rs1 - {R1})"
+  assumes k: "NT N \<notin> NonTerminals G1"
+  shows      "TermMeasure G1 > TermMeasure G2"
+proof-
+  from c have "CountNonSingleTerminals R3 = 0" by simp
+  from a and b and d have "CountNonSingleTerminals R1 = CountNonSingleTerminals R2 + 1"
+    by (meson CountProperty2)
+  
+theorem TermTerminate:
+  assumes a: "transformTermSingle G1 N G2"
+  assumes b: "finiteCFG G1"
+  shows      "TermMeasure G1 > TermMeasure G2"
+proof-
+  from a and b and TermFinite have 0: "finiteCFG G2" 
+    by metis
+  from a have 1: "\<exists> S R1 R2 R3 Rs1 Rs2 S1 L R a. 
+                    (S, Rs1) = G1 
+                    \<and> R1 = (S1, L @ (T(a) # R))
+                    \<and> R2 = (S1, L @ (NT(N) # R))
+                    \<and> R3 = (N, [T a])
+                    \<and> (L @ R \<noteq> [])
+                    \<and> (S, Rs2) = G2 
+                    \<and> R1 \<in> Rs1
+                    \<and> Rs2 = {R2, R3} \<union> (Rs1 - {R1})
+                    \<and> NT(N) \<notin> NonTerminals(G1)" 
+                  (is "\<exists>S R1 R2 R3 Rs1 Rs2 S1 L R a. ?P S R1 R2 R3 Rs1 Rs2 S1 L R a")
+    by (simp add: transformTermSingle_def)
+  from 1 obtain S R1 R2 R3 Rs1 Rs2 S1 L R a where 2: "?P S R1 R2 R3 Rs1 Rs2 S1 L R a" by blast
+  from 2 have 3: "CountNonSingleTerminals R3 = 0"
+    by simp
+  from 2 have 4: "CountNonSingleTerminals R1 = CountNonSingleTerminals R2 + 1"
+    by (meson CountProperty2)
 end
